src/ProbabilisticProgramming/Monad.dfy
@@ -16,14 +16,51 @@ module Monad {
   type Hurd<A> = Rand.Bitstream -> Result<A>
 
   // The result of a probabilistic computation on a bitstream.
-  // It consists of the computed value and the (unconsumed) rest of the bitstream.
-  datatype Result<A> = Result(value: A, rest: Rand.Bitstream)
+  // It either consists of the computed value and the (unconsumed) rest of the bitstream or indicates nontermination.
+  datatype Result<A> =
+  | Result(value: A, rest: Rand.Bitstream)
+  | Diverging
+{
+  function Map<B>(f: A -> B): Result<B> {
+    match this
+    case Diverging => Diverging
+    case Result(value, rest) => Result(f(value), rest)
+  }
+
+  function Bind<B>(f: A -> Hurd<B>): Result<B> {
+    match this
+    case Diverging => Diverging
+    case Result(value, rest) => f(value)(rest)
+  }
+
+  ghost predicate In(s: iset<A>) {
+    Satisfies(x => x in s)
+  }
+
+  ghost predicate Equals(a: A) {
+    Satisfies(x => x == a)
+  }
+
+  predicate Satisfies(property: A -> bool) {
+    match this
+    case Diverging => false
+    case Result(value, _) => property(value)
+  }
+
+  ghost predicate RestIn(s: iset<Rand.Bitstream>) {
+    RestSatisfies(r => r in s)
+  }
+
+  predicate RestSatisfies(property: Rand.Bitstream -> bool) {
+    match this
+    case Diverging => false
+    case Result(_, rest) => property(rest)
+  }
+}
 
   // Equation (3.4)
   function Bind<A,B>(f: Hurd<A>, g: A -> Hurd<B>): Hurd<B> {
-    (s: Rand.Bitstream) =>
-      var Result(a, s') := f(s);
-      g(a)(s')
+    (s: Rand.Bitstream) => f(s).Bind(g)
   }
 
   // Equation (2.42)
@@ -38,14 +75,12 @@ module Monad {
     (s: Rand.Bitstream) => Result(a, s)
   }
 
-  function Map<A,B>(f: A -> B, m: Hurd<A>): Hurd<B> {
+  function Map<A,B>(m: Hurd<A>, f: A -> B): Hurd<B> {
     Bind(m, (a: A) => Return(f(a)))
   }
 
   function Join<A>(ff: Hurd<Hurd<A>>): Hurd<A> {
-    (s: Rand.Bitstream) =>
-      var Result(f, s') := ff(s);
-      f(s')
+    (s: Rand.Bitstream) => ff(s).Bind(f => f)
   }
 
   /*******
@@ -58,49 +93,18 @@ module Monad {
 
   lemma BindIsAssociative<A,B,C>(f: Hurd<A>, g: A -> Hurd<B>, h: B -> Hurd<C>, s: Rand.Bitstream)
     ensures Bind(Bind(f, g), h)(s) == Bind(f, (a: A) => Bind(g(a), h))(s)
-  {
-    var Result(a, s') := f(s);
-    var Result(a', s'') := g(a)(s');
-    assert Result(a', s'') == Bind(f, g)(s);
-    calc {
-      Bind(Bind(f, g), h)(s);
-      h(a')(s'');
-      Bind(g(a), h)(s');
-      Bind(f, (a: A) => Bind(g(a), h))(s);
-    }
-  }
+  {}
 
   lemma CompositionIsAssociative<A,B,C,D>(f: A -> Hurd<B>, g: B -> Hurd<C>, h: C -> Hurd<D>, a: A, s: Rand.Bitstream)
     ensures Composition(Composition(f, g), h)(a)(s) == Composition(f, Composition(g, h))(a)(s)
-  {
-    BindIsAssociative(f(a), g, h, s);
-  }
+  {}
 
   lemma UnitalityJoinReturn<A>(f: Hurd<A>, s: Rand.Bitstream)
-    ensures Join(Map(Return, f))(s) == Join(Return(f))(s)
-  {
-    var Result(a, t) := f(s);
-    calc {
-      Join(Return(f))(s);
-    ==
-      Result(a, t);
-    ==
-      Join(Map(Return, f))(s);
-    }
-  }
+    ensures Join(Map(f, Return))(s) == Join(Return(f))(s)
+  {}
 
   lemma JoinIsAssociative<A>(fff: Hurd<Hurd<Hurd<A>>>, s: Rand.Bitstream)
-    ensures Join(Map(Join, fff))(s) == Join(Join(fff))(s)
-  {
-    var Result(ff, t) := fff(s);
-    var Result(f, u) := ff(t);
-    calc {
-      Join(Map(Join, fff))(s);
-    ==
-      f(u);
-    ==
-      Join(Join(fff))(s);
-    }
-  }
+    ensures Join(Map(fff, Join))(s) == Join(Join(fff))(s)
+  {}
 }
 
