src/Distributions/UniformPowerOfTwo/Model.dfy
@@ -23,6 +23,7 @@ module UniformPowerOfTwo.Model {
   // The return value u is uniformly distributed between 0 <= u < 2^k where 2^k <= n < 2^(k + 1).
   opaque function Sample(n: nat): (h: Monad.Hurd<nat>)
     requires n >= 1
+    ensures forall s :: Sample(n)(s).Result? // always terminates, not just almost surely
   {
     if n == 1 then
       Monad.Return(0)
